C11-FrontEnd/examples/C_paper.thy
@@ -55,7 +55,7 @@ val C' = C_Module.C'
 fun C_define dir name _ _ =
   Context.map_theory 
     (C_Inner_Syntax.command0
-      (fn src => fn context => C' (C_Stack.Data_Lang.get context |> #2) src context)
+      (fn src => fn context => C' (C_Stack.Data_Lang.get' context |> #2) src context)
       C_Parse.C_source
       dir
       name)
